왘ㅋㅋㅋㅋㅋㅋ 증명하다가 자체적으로 '버그'를 '잡았' 어 ㅋㅋㅋㅋㅋㅋ

src/common/Nemonuri.IndexSet.Invariant.fst
@@ -19,16 +19,31 @@ let empty : t = {
   count = 0; set = FSet.emptyset #int
 }
 
+(*
 let lemma_insert (s:t) (x:int)
   : Lemma ((I.interval_condition 0 (s.count+1) x) <==> (FSet.mem x (FSet.insert (s.count+1) s.set)))
   =
-  ()
-
-(*
-let push (s:t) : Tot t =
-  let next_count = s.count + 1 in
-  {
-    count = next_count;
-    set = FSet.insert next_count s.set
-  }
+  let lhs = (I.interval_condition 0 (s.count+1) x) in
+  let rhs = (FSet.mem x (FSet.insert (s.count+1) s.set)) in
+  let lemma_l_to_r' () : Lemma (lhs ==> rhs) =
+    match lhs with
+    | false -> () | true ->
+    match (I.interval_condition 0 s.count x) with
+    | true -> assert (FSet.mem x s.set) | false ->
+    assert 
+  in
+  let lemma_r_to_l' () : Lemma (rhs ==> lhs) =
+    admit ()
+  in
+  lemma_l_to_r' ();
+  lemma_r_to_l' ()
 *)
+
+module C = FStar.Classical
+
+let push (s:t) : Tot t =
+  //C.forall_intro (lemma_insert s);
+  {
+    count = s.count + 1;
+    set = FSet.insert s.count s.set
+  }
